backends/lean-iris/AeneasIris.lean
@@ -8,10 +8,10 @@ import AeneasIris.HeapAPI
 import AeneasIris.RwLock
 import AeneasIris.RwLockLAT
 import AeneasIris.Arc
+import AeneasIris.ArcLAT
 import AeneasIris.RustHandler
 import AeneasIris.ISpec
 import AeneasIris.Triple
-import AeneasIris.Primitives
 import AeneasIris.Tactics
 import AeneasIris.ConcurrencyAPI
 import AeneasIris.Zoo
